correctness/RegexCorrectness/Syntax/Ast.lean
@@ -30,16 +30,10 @@ theorem repeatConcat_tags (e : Expr) (n : Nat) : (repeatConcat e n).tags = e.tag
   . simpa using repeatConcat_go_tags_subset e e (n - 1)
   . exact subset_repeatConcat_go_tags e e (n - 1) (by simp)
 
-theorem applyRepetitions_tags (min : Nat) (max : Option Nat) (e : Expr) :
-  (applyRepetitions min max e).tags ⊆ e.tags := by
+theorem applyRepetitions_tags (min : Nat) (max : Option Nat) (greedy : Bool) (e : Expr) :
+  (applyRepetitions min max greedy e).tags ⊆ e.tags := by
   simp only [applyRepetitions]
-  split
-  · simp [Expr.tags]
-  · simp [Expr.tags]
-  · simp [Expr.tags]
-  · simp [Expr.tags, repeatConcat_tags]
-  · split <;> simp [Expr.tags, repeatConcat_tags]
-  · split <;> simp [Expr.tags, repeatConcat_tags]
+  grind [Expr.tags, repeatConcat_tags]
 
 -- `Finset.ico index index'` corresponds to a half-open interval [index, index').
 theorem toRegexAux_tags {index index' : Nat} {ast : Ast} {e : Expr}
@@ -79,11 +73,11 @@ theorem toRegexAux_tags {index index' : Nat} {ast : Ast} {e : Expr}
     have ⟨le₂, ih₂⟩ := ih₂ h₂
     simp [←h, Expr.tags]
     exact ⟨Nat.le_trans le₁ le₂, Finset.Ico_union_Ico_eq_Ico le₁ le₂ ▸ Finset.union_subset_union ih₁ ih₂⟩
-  next index min max ast index'' e' h' ih =>
+  next index min max greedy ast index'' e' h' ih =>
     simp at h
     have ⟨le, ih⟩ := ih h'
     simp [←h, le]
-    exact Finset.Subset.trans (applyRepetitions_tags min max e') ih
+    exact Finset.Subset.trans (applyRepetitions_tags min max greedy e') ih
   next =>
     simp at h
     simp [←h, Expr.tags]
@@ -103,9 +97,9 @@ theorem repeatConcat_go_disjoint (e : Expr) (accum : Expr) (n : Nat) (h : e.Disj
 theorem repeatConcat_disjoint (e : Expr) (n : Nat) (h : e.Disjoint) : (repeatConcat e n).Disjoint :=
   repeatConcat_go_disjoint e e (n - 1) h h
 
-theorem applyRepetitions_disjoint (min : Nat) (max : Option Nat) (e : Expr) (h : e.Disjoint) :
-  (applyRepetitions min max e).Disjoint := by
-  fun_cases applyRepetitions min max e <;> simp_all [Expr.Disjoint, repeatConcat_disjoint]
+theorem applyRepetitions_disjoint (min : Nat) (max : Option Nat) (greedy : Bool) (e : Expr) (h : e.Disjoint) :
+  (applyRepetitions min max greedy e).Disjoint := by
+  fun_cases applyRepetitions min max greedy e <;> grind [Expr.Disjoint, repeatConcat_disjoint]
 
 theorem toRegexAux_disjoint (index : Nat) (ast : Ast) : Expr.Disjoint (ast.toRegexAux index).2 := by
   fun_induction ast.toRegexAux index
@@ -123,9 +117,9 @@ theorem toRegexAux_disjoint (index : Nat) (ast : Ast) : Expr.Disjoint (ast.toReg
   next index ast₁ ast₂ index₁ e₁ h₁ index₂ e₂ h₂ ih₁ ih₂ =>
     simp [h₁, h₂] at ih₁ ih₂
     simp [Expr.Disjoint, ih₁, ih₂]
-  next index min max ast index' e h ih =>
+  next index min max greedy ast index' e h ih =>
     simp [h] at ih
-    exact applyRepetitions_disjoint min max e ih
+    exact applyRepetitions_disjoint min max greedy e ih
   next => simp [Expr.Disjoint]
   next => simp [Expr.Disjoint]
   next => simp [Expr.Disjoint]
